Lean/Egg/Core/Encode/Basic.lean
@@ -20,12 +20,15 @@ private def encodeLevel (src : Source) : Level → EncodeM Expression
   | .succ l     => return s!"(succ {← encodeLevel src l})"
   | .max l₁ l₂  => return s!"(max {← encodeLevel src l₁} {← encodeLevel src l₂})"
   | .imax l₁ l₂ => return s!"(imax {← encodeLevel src l₁} {← encodeLevel src l₂})"
+  -- TODO: This should check whether the level mvar is ambient, just as for expression mvars.
+  --       Once we do this, we can also remove `exprSrc` from the monad state.
   | .mvar id    => return if src.isRewrite then s!"?{id.uniqueIdx!}" else s!"(uvar {id.uniqueIdx!})"
   | .param name => return s!"(param {name})"
 
 -- Note: This function expects its input expression to be normalized (cf. `Egg.normalize`).
-partial def encode (e : Expr) (src : Source) (cfg : Config.Encoding) : MetaM Expression :=
-  Prod.fst <$> (go e).run { exprSrc := src, config := cfg }
+partial def encode (e : Expr) (src : Source) (cfg : Config.Encoding) (amb : MVars.Ambient) :
+    MetaM Expression :=
+  Prod.fst <$> (go e).run { exprSrc := src, config := cfg, amb }
 where
   go (e : Expr) : EncodeM Expression := do
     if ← needsProofErasure e then return Expression.erased else core e
@@ -49,9 +52,9 @@ where
     else return s!"(fvar {id.uniqueIdx!})"
 
   encodeMVar (id : MVarId) : EncodeM Expression := do
-    if (← exprSrc).isRewrite
-    then return s!"?{id.uniqueIdx!}"
-    else return s!"(mvar {id.uniqueIdx!})"
+    if (← isAmbient id)
+    then return s!"(mvar {id.uniqueIdx!})"
+    else return s!"?{id.uniqueIdx!}"
 
   encodeConstLvls (lvls : List Level) : EncodeM Expression :=
     lvls.foldlM (init := "") (return s!"{·} {← encodeLevel (← exprSrc) ·}")
