Lean/Egg/Core/Encode/Rewrites.lean
@@ -12,11 +12,11 @@ structure Rewrite.Encoded where
   rhs  : Expression
   dirs : Directions
 
-def Rewrite.encode (cfg : Config.Encoding) (rw : Rewrite) : MetaM Encoded :=
+def Rewrite.encode (rw : Rewrite) (cfg : Config.Encoding) (amb : MVars.Ambient) : MetaM Encoded :=
   return {
     name := rw.src.description
-    lhs  := ← Egg.encode rw.lhs rw.src cfg
-    rhs  := ← Egg.encode rw.rhs rw.src cfg
+    lhs  := ← Egg.encode rw.lhs rw.src cfg amb
+    rhs  := ← Egg.encode rw.rhs rw.src cfg amb
     dirs := rw.validDirs
   }
 
@@ -24,5 +24,5 @@ namespace Rewrites
 
 abbrev Encoded := Array Rewrite.Encoded
 
-def encode (rws : Rewrites) (cfg : Config.Encoding) : MetaM Rewrites.Encoded :=
-  rws.mapM (Rewrite.encode cfg)
+def encode (rws : Rewrites) (cfg : Config.Encoding) (amb : MVars.Ambient) : MetaM Rewrites.Encoded :=
+  rws.mapM (·.encode cfg amb)
