Lean/Egg/Core/MVars/Ambient.lean
@@ -1,0 +1,19 @@
+import Egg.Core.MVars.Basic
+import Lean
+open Lean
+
+namespace Egg.MVars
+
+abbrev Ambient := MVarIdSet
+
+def Ambient.get : MetaM Ambient := do
+  let mut result := ∅
+  for (mvar, _) in (← getMCtx).decls do
+    if !(← mvar.isAssigned) then
+      result := result.insert mvar
+  return result
+
+def remove (mvars : MVars) (amb : Ambient) : MVars where
+  expr := mvars.expr.filter (!amb.contains ·)
+  lvl  := mvars.lvl
+  tc   := mvars.tc.filter (!amb.contains ·)
