Lean/Egg/Core/MVars/Subst.lean
@@ -1,0 +1,71 @@
+import Egg.Core.MVars.Basic
+import Lean
+open Lean Meta
+
+namespace Egg.MVars
+
+protected structure Subst.Expr where
+  fwd : HashMap MVarId MVarId := ∅
+  bwd : HashMap MVarId MVarId := ∅
+
+protected abbrev Subst.Lvl := HashMap LMVarId LMVarId
+
+structure Subst where
+  expr : Subst.Expr := {}
+  lvl  : Subst.Lvl  := ∅
+
+def Subst.apply (subst : Subst) (e : Expr) : Expr :=
+  e.replace replaceExpr
+where
+  replaceExpr : Expr → Option Expr
+  | .mvar id         => subst.expr.fwd.find? id >>= (Expr.mvar ·)
+  | .sort lvl        => Expr.sort <| lvl.replace replaceLvl
+  | .const name lvls => Expr.const name <| lvls.map (·.replace replaceLvl)
+  | _                => none
+
+  replaceLvl : Level → Option Level
+  | .mvar id => subst.lvl.find? id >>= (Level.mvar ·)
+  | _        => none
+
+def fresh (mvars : MVars) (init : Subst := {}) : MetaM (MVars × Subst) := do
+  let (exprVars, exprSubst) ← freshExprs mvars.expr init.expr
+  let (lvlVars, lvlSubst) ← freshLvls mvars.lvl init.lvl
+  let subst := { expr := exprSubst, lvl := lvlSubst }
+  assignFreshExprMVarTypes exprVars subst
+  return ({ expr := exprVars, lvl := lvlVars }, subst)
+where
+  freshExprs (src : MVarIdSet) (subst : Subst.Expr) : MetaM (MVarIdSet × Subst.Expr) := do
+    let mut vars : MVarIdSet := {}
+    let mut subst := subst
+    for var in src do
+      if let some f := subst.fwd.find? var then
+        vars := vars.insert f
+      else
+        -- Note: As the type of an mvar may also contain mvars, we also have to replace mvars with
+        --       their fresh counterpart *in the type*. We can only do this once we know the fresh
+        --       counterpart for each mvar, so we postpone the type assignment.
+        let f ← mkFreshExprMVar none
+        subst := {
+          fwd := subst.fwd.insert var f.mvarId!
+          bwd := subst.bwd.insert f.mvarId! var
+        }
+        vars := vars.insert f.mvarId!
+    return (vars, subst)
+
+  freshLvls (src : LMVarIdSet) (subst : Subst.Lvl) : MetaM (LMVarIdSet × Subst.Lvl) := do
+    let mut vars : LMVarIdSet := {}
+    let mut subst := subst
+    for var in src do
+      if let some f := subst.find? var then
+        vars := vars.insert f
+      else
+        let f ← mkFreshLevelMVar
+        subst := subst.insert var f.mvarId!
+        vars := vars.insert f.mvarId!
+    return (vars, subst)
+
+  assignFreshExprMVarTypes (vars : MVarIdSet) (subst : Subst) : MetaM Unit := do
+    for var in vars do
+      let srcType ← (subst.expr.bwd.find! var).getType
+      let freshType := subst.apply srcType
+      var.setType freshType
