Lean/Egg/Tests/Ambient MVar.lean
@@ -1,0 +1,19 @@
+import Egg
+import Lean
+
+example (h : ∀ x : Prop, True = x) : True = True := by
+  apply Eq.trans
+  · egg [h]
+  · rfl -- This assigns the mvar resulting from `Eq.trans`.
+
+/--
+error: unsolved goals
+case b
+h : ∀ (x : Prop), True = x
+⊢ Prop
+-/
+#guard_msgs in
+example (h : ∀ x : Prop, True = x) : True = True := by
+  apply Eq.trans
+  · egg [h]
+  · egg [h]
