Lean/Egg/Tests/Loose Argument.lean
@@ -1,0 +1,6 @@
+import Egg
+
+/-- error: Rewrite #0 contains loose argument. -/
+#guard_msgs in
+example (h : ∀ n : Nat, n > 2 → n = 5) : x = 5 := by
+  egg [h]
